src/lowparse/pulse/LowParse.Pulse.Int.fst
@@ -39,6 +39,10 @@ inline_for_extraction
 let read_u8 : reader tot_serialize_u8 = reader_of_leaf_reader (read_u8' ())
 
 inline_for_extraction
+let validate_and_read_u8 : validate_and_read tot_parse_u8 =
+  validate_and_read_intro validate_u8 read_u8
+
+inline_for_extraction
 let validate_u16 : validator tot_parse_u16 =
   validate_total_constant_size tot_parse_u16 2sz
 
@@ -67,6 +71,10 @@ fn read_u16' (_: unit) : leaf_reader #FStar.UInt16.t #parse_u16_kind #tot_parse_
 
 inline_for_extraction
 let read_u16 : reader tot_serialize_u16 = reader_of_leaf_reader (read_u16' ())
+
+inline_for_extraction
+let validate_and_read_u16 : validate_and_read tot_parse_u16 =
+  validate_and_read_intro validate_u16 read_u16
 
 inline_for_extraction
 let validate_u32 : validator tot_parse_u32 =
@@ -99,6 +107,10 @@ inline_for_extraction
 let read_u32 : reader tot_serialize_u32 = reader_of_leaf_reader (read_u32' ())
 
 inline_for_extraction
+let validate_and_read_u32 : validate_and_read tot_parse_u32 =
+  validate_and_read_intro validate_u32 read_u32
+
+inline_for_extraction
 let validate_u64 : validator tot_parse_u64 =
   validate_total_constant_size tot_parse_u64 8sz
 
@@ -127,3 +139,7 @@ fn read_u64' (_: unit) : leaf_reader #FStar.UInt64.t #parse_u64_kind #tot_parse_
 
 inline_for_extraction
 let read_u64 : reader tot_serialize_u64 = reader_of_leaf_reader (read_u64' ())
+
+inline_for_extraction
+let validate_and_read_u64 : validate_and_read tot_parse_u64 =
+  validate_and_read_intro validate_u64 read_u64
